Fomega/Basic/Classification.lean
@@ -8,40 +8,38 @@ import Fomega.Basic.Inversion
 
 namespace Fomega.Proof
 
-  theorem proof_classification : t ⊢ Γ -> Γ ⊢ t : A -> A = □ ∨ (∃ K, Γ ⊢ A : .const K) := by
-  intro j1 j2
-  induction j2
+  theorem proof_classification : Γ ⊢ t : A -> A = □ ∨ (∃ K, Γ ⊢ A : .const K) := by
+  intro j
+  induction j
   case ax => apply Or.inl; rfl
-  case var Γ K x =>
-    apply Or.inr; cases j1
-    case _ j => exists K
-  case pi =>
-    apply Or.inr
-    exists .kind; constructor
+  case var K h _ => apply Or.inr; exists K
+  case pi h _ _ _ =>
+    have h2 := ctx_wf h
+    cases h2
+    case _ f h2 =>
+      apply Or.inr; exists .kind; apply Proof.ax f h2
   case tpi => apply Or.inl; rfl
   case lam h1 _h2 _ih1 _ih2 => apply Or.inr; apply Exists.intro; apply h1
   case app _h1 h2 h3 ih1 _ih2 =>
-    cases j1
-    case _ j1 j2 =>
-      replace ih1 := ih1 j1
-      cases ih1 <;> simp at *
-      case _ h =>
+    replace ih1 := ih1
+    cases ih1 <;> simp at *
+    case _ h =>
+      cases h
+      case _ K h =>
         cases h
-        case _ K h =>
-          cases h
-          case _ K q1 q2 =>
-            have h := Proof.beta q2 h2; simp at h
-            apply Or.inr; exists .type
-            subst h3; exact h
-          case _ K q1 q2 =>
-            have h := Proof.beta q2 h2; simp at h
-            apply Or.inr; exists .kind
-            subst h3; exact h
-          case _ C K' q1 q2 q3 =>
-            replace q1 := all_destruct q1 q2
-            have h := Proof.beta (q1.2.2) h2
-            simp at h; apply Or.inr; exists K
-            subst h3; apply h
+        case _ K q1 q2 =>
+          have h := Proof.beta q2 h2; simp at h
+          apply Or.inr; exists .type
+          subst h3; exact h
+        case _ K q1 q2 =>
+          have h := Proof.beta q2 h2; simp at h
+          apply Or.inr; exists .kind
+          subst h3; exact h
+        case _ C K' q1 q2 q3 =>
+          replace q1 := all_destruct q1 q2
+          have h := Proof.beta (q1.2.2) h2
+          simp at h; apply Or.inr; exists K
+          subst h3; apply h
   case iconv K _h1 h2 _h3 _ih1 _ih2 =>
     apply Or.inr; exists K
   case econv K _h1 h2 _h3 _ih1 _ih2 =>
